shitpost

Notes/Chapter7/Sec2Bob.lean
@@ -1,5 +1,227 @@
 /- @file Notes/Chapter7/Sec2Bob.lean
  - @src https://lean-lang.org/functional_programming_in_lean/monad-transformers/transformers.html
  -/
+namespace ν
 
-/- SECTION: -/
+/- SECTION: What is a Monad Transformer? -/
+
+-- A monad transformer consists of the following:
+-- [1.] A definition/datatype `T` that takes a monad as an argument.
+--   Its type should be `⋯ → (Type u → Type v) → Type u → Type v`.
+-- [2.] A `Monad` instance for `T m` which relies on a `[Monad m]` instance.
+-- [3.] A `MonadLift m (T m)` instance that translates actions `: m α` to actions
+--   `: T m α`.
+-- Furthermore, all the relevant stuff should be `Lawful`:
+-- [4.] There should be a proof `: [LawfulMonad m] → [LawfulMonad (T m)]`.
+-- [5.] `∀ x, monadLift ((pure (m := m)) x) = (pure (m := T m)) x`
+-- [6.] `∀ x f, monadLift (x >>= f) = monadLift x >>= (monadLift ∘ f)`
+
+
+
+/- SECTION: `OptionT`, and a sample program for it -/
+
+-- [1.] Definition of `OptionT`
+abbrev OptionT  : (Type u → Type v) → Type u → Type v := (· ∘ Option)
+def OptionT.mk  : m (Option α) → OptionT m α := id
+def OptionT.run : OptionT m α → m (Option α) := id
+
+-- [2.]
+def OptionT.pure [Monad m] : α → OptionT m α
+  | a => (Pure.pure (f := m)) (some a)
+  -- Alternatively, `(Pure.pure (some a) : m (Option _))`
+
+-- [2.]
+def OptionT.bind [Monad m] : OptionT m α → (α → OptionT m β) → OptionT m β :=
+  fun moa f =>
+    (Bind.bind (m := m)) moa <| fun oa =>
+      match oa with
+      | none   => (Pure.pure (f := m)) none
+      | some a => f a
+
+-- [2.] Promoting `Monad` instances
+instance [Monad m] : Monad (OptionT m) where
+  pure := OptionT.pure
+  bind := OptionT.bind
+
+-- [3.] A `MonadLift` instance
+instance [Monad m] : MonadLift m (OptionT m) where
+  -- `: m α → OptionT m α`
+  monadLift := fun ma =>
+    (Functor.map (f := m)) some ma
+
+-- [4.]
+theorem OptionT.id_map.{u_1}
+  [Monad m] [law : LawfulMonad m]
+  : ∀ {α : Type u_1} (x : OptionT m α), id <$> x = x
+  := sorry
+  -- by
+  --   intro α moa
+  --   show OptionT.bind moa (pure ∘ id) = moa
+  --   have comp_id : ∀ {β : Type u_1} {γ : Type u_2} (f : β → γ), f ∘ id = f := by
+  --     intros
+  --     funext
+  --     rfl
+  --   rw [comp_id]
+  --   unfold OptionT.bind
+  --   have match_pure_comm
+  --     : ∀ (oa : Option α),
+  --       (match oa with | none => pure none | some a => pure a) = (pure oa : m (Option α))
+  --     := by
+  --       intro oa ; cases oa <;> rfl
+  --   show (Bind.bind (m := m)) moa (fun (oa : Option α) => match oa with | none => pure none | some a => pure a)
+  --     = moa
+  --   conv => { lhs; rhs; intro; rw [match_pure_comm] }
+  --   show moa.run >>= pure = moa.run
+  --   have : (id : Option α → Option α) = (fun a => a) := rfl
+  --   rw [law.bind_pure_comp]
+  --   have it := law.id_map (α := Option α)
+  --   rw [this] at it
+  --   rw [it]
+
+-- [4.] Check `LawfulMonad` gets inherited
+instance [Monad m] [law : LawfulMonad m] : LawfulMonad (OptionT m) where
+  map_const := rfl
+  id_map := OptionT.id_map -- pain in the ass
+  seqLeft_eq := sorry -- fuck this
+  seqRight_eq := sorry -- fuck this
+  pure_seq := sorry -- fuck this
+  bind_pure_comp := sorry -- fuck this
+  bind_map := sorry -- fuck this
+  pure_bind := sorry -- fuck this
+  bind_assoc := sorry -- FUCK this
+
+-- [5.], [6.]: cba
+instance [Monad m] : MonadLift m (OptionT m) where
+  monadLift action := OptionT.mk do
+    pure (some (← action))
+
+instance [Monad m] : Alternative (OptionT m) where
+  failure := OptionT.mk (pure none)
+  orElse x ly := OptionT.mk do
+    match ← x with
+    | none        => ly ()
+    | some result => pure (some result)
+
+def getSomeInput : OptionT IO String := do
+  let input ← (← IO.getStdin).getLine
+  let trimmed := input.trim
+  if trimmed == "" then
+    failure
+  else pure trimmed
+
+structure UserInfo where
+  name         : String
+  favouriteCat : String
+
+def getUserInfo : OptionT IO UserInfo := do
+  IO.println "Give name"
+  let name ← getSomeInput
+  IO.println "Give favourite cat"
+  let cat ← getSomeInput
+  pure ⟨name, cat⟩
+
+def interact : IO Unit := do
+  match ← getUserInfo with
+  | none => IO.eprintln "Damnit dude"
+  | some ⟨name, cat⟩ => IO.println s!"Hi {name} who likes {cat}"
+
+
+
+/- SECTION: `ExceptT` -/
+
+-- This is pretty much the same as `OptionT`. `ExceptT PUnit` is isomorphic to `OptionT`.
+def ExceptT (ε : Type u) (m : Type u → Type v) : Type u → Type v := m ∘ Except ε
+
+def ExceptT.mk  {ε α : Type u} (mea : m (Except ε α)) : ExceptT ε m α  := mea
+def ExceptT.run {ε α : Type u} (ema : ExceptT ε m α)  : m (Except ε α) := ema
+
+instance
+  {ε : Type u} {m : Type u → Type v} [Monad m]
+  : Monad (ExceptT ε m)
+  where
+    pure a := ExceptT.mk (pure (Except.ok a))
+    bind mea f := ExceptT.mk do
+      match ← mea with
+      | .ok    a => f a
+      | .error e => pure (.error e)
+
+instance [Monad m] : MonadLift (Except ε) (ExceptT ε m) where
+  monadLift ea := ExceptT.mk (pure ea)
+
+instance [Monad m] : MonadLift m (ExceptT ε m) where
+  monadLift ma := ExceptT.mk <| .ok <$> ma
+    -- This is what I came up with; it's probably existentially equivalent:
+    -- `ExceptT.mk do         `
+    -- `  (pure ∘ .ok) (← ma) `
+
+
+
+/- SECTION: `MonadExcept` -/
+
+/- Lean supports
+  ` class MonadExcept (ε : outParam (Type u)) (m : Type v → Type w) where `
+  `   throw    : ε → m α                                                  `
+  `   tryCatch : m α → (ε → m α) → m α                                    `
+-/
+
+inductive Err where
+  | divByZero : Err
+  | nAN       : String → Err
+
+def divBackend [Monad m] [MonadExcept Err m] (n d : Int) : m Int :=
+  if d = 0 then throw .divByZero else pure (n / d)
+
+def asNumber [Monad m] [MonadExcept Err m] (s : String) : m Int :=
+  match s.toInt? with
+  | none   => throw (.nAN s)
+  | some i => pure i
+
+def divFrontend [Monad m] [MonadExcept Err m] (n d : String) : m String := do
+  try
+    pure (toString (← divBackend (← asNumber n) (← asNumber d)))
+  catch
+    | .divByZero => pure "Fuck mate, you divided by zero; no bueno bruda"
+    | .nAN s     => pure s!"Mate, {s} is not a numba"
+-- Here, `try (t : m α) catch (c : ε → m α)` is sugar for `tryCatch t c`
+
+
+
+/- SECTION: `StateT` -/
+
+def StateT (σ : Type u) (m : Type u → Type v) : Type u → Type (max u v) :=
+  fun α => σ → m (α × σ)
+
+instance [Monad m] : Monad (StateT σ m) where
+  pure a := fun s => pure (a, s)
+  bind sma f :=
+    fun s => do
+      let (a, s') ← sma s
+      f a s'
+
+-- Lean supports these:
+/-
+  ` class MonadState                  `
+  `   (σ : outParam (Type u))         `
+  `   (m : Type u → Type v)           `
+  `   : Type (max (u + 1) v) where    `
+  `     get : m σ                     `
+  `     set : σ → m PUnit             `
+  `     modifyGet : (σ → α × σ) → m α `
+-- and this, which uses `modifyGet` without actually providing a meaningful return value:
+  ` def modify.{u, v}                         `
+  `   : {σ : Type u}                          `
+  `   → {m : Type u → Type v}                 `
+  `   → [inst : MonadState σ m]               `
+  `   → (σ → σ)                               `
+  `   → m PUnit                               `
+  `   := fun {σ} {m} [MonadState σ m] f =>    `
+  `     modifyGet fun s => (PUnit.unit, f s)  `
+-/
+#print modify
+
+
+
+end ν
+/- LAUNCH: -/
+
+def main : IO Unit := ν.interact
